Proof/Algorithm/EndsInFixPoint.lean
@@ -2,10 +2,31 @@ import Proof.Algorithm.Definition
 
 namespace Algorithm
 
-open Proof (Program)
+open Proof (Program GlobName Expr)
+
+theorem every_object_is_in_fixpoint {L : Program} {hL : L.HasMain} {G : GlobName}
+    {e₁ e₂ : Expr} {F : FixPoints} (hG : L.HasObject G e₁ e₂)
+    (hC : Solve.Star L (Config.start L hL) (.done F))
+    : InFixPoint F G := by
+  sorry
+
+theorem fixpoint_is_stable {c : Config} {G : GlobName}
+    {L : Program} (h : InFixPoint c.fixpoints G)
+    : Stable L c.fixpoints G (c.fixpoints.lookup G h) := by
+  sorry
 
 theorem solve_done_fixpoint {L : Program} {F : FixPoints} {hL : L.HasMain}
     (h : Solve.Star L (Config.start L hL) (.done F)) : Proof.FixPoint F.glue L := by
-  sorry
+  refine ⟨?_, ?_, ?_, ?_, ?_, ?_, ?_, ?_⟩
+  · -- rm_init
+    intro G e₁ e₂ K₁ K₂ hG hCe₁ hCe₂
+    sorry
+  · sorry
+  · sorry
+  · sorry
+  · sorry
+  · sorry
+  · sorry
+  · sorry
 
 end Algorithm
