README.md
@@ -10,3 +10,13 @@ Next steps:
 
 Date: Sept 18
 Looked at LessThanInv. It makes sense.
+Added a termination theorem in Termination.lean
+Started EndsInFixPoint by first proving that every state G in the fixpoint is
+stable, which gives us Grow, and thus FixPoint
+We also need the helper that every_object_is_in_fixpoint, by virtue to config.start
+(This is probably different from what the algorithm actually does though...
+
+If Instead, config.start doesn't have a queue at all. We only suspend and resume...
+Then we need to say that every object that Main depends on (the algorithm's Dep) is InFixPoint
+...but how?
+)
